Adding more stuff in CPS.

theories/misc/CPS.v
@@ -38,6 +38,12 @@ Definition Cᴿ (A : TYPE) : (C A -> Ω) -> Type :=
 
 Definition El (A : TYPE) : Type := sig (C A -> Ω) (Cᴿ A).
 
+Inductive Freeᴿ {A} : M A -> Type :=
+| freeᴿ : forall x, Freeᴿ (ret x).
+
+Definition Free (A : Type) : TYPE :=
+  exist (M Type) Typeᴿ (ret (A -> Ω)) (IsType _ Freeᴿ).
+
 Check Typeᶠ : El Typeᶠ.
 
 Definition Prodᶠ (A : TYPE) (B : El A -> TYPE) : El Typeᶠ.
@@ -121,7 +127,7 @@ refine (λᶠ A x, _).
 unshelve refine (exist _ _ x.(wit) tt).
 Defined.
 
-Lemma cc : El (Πᶠ (A B : El Typeᶠ), ((A →ᶠ [[ B ]]) →ᶠ A) →ᶠ [[ A ]]).
+Lemma cc : El (Πᶠ (A B : El Typeᶠ), ((A →ᶠ [[ B ]]) →ᶠ [[ A ]]) →ᶠ [[ A ]]).
 Proof.
 refine (λᶠ A B f, _).
 simple refine (exist _ _ (fun ω => _) _).
@@ -162,6 +168,49 @@ intros P Pt Pf; compute.
 destruct Pf as [? [ ] ]; reflexivity.
 Defined.
 
+Lemma squash_bool_case_cc : forall P X (M : El ((boolᶠ →ᶠ [[ X ]]) →ᶠ [[ boolᶠ ]])) Pt Pf,
+  squash_bool_caseᶠ · P · Pt · Pf · (cc · boolᶠ · X · M) =
+  cc · [[ P ]] · X · (λᶠ (k : El ([[ P ]] →ᶠ [[ X ]])),
+    squash_bool_caseᶠ · P · Pt · Pf ·
+      (M · (λᶠ (x : El boolᶠ),
+        k · (squash_bool_caseᶠ · P · Pt · Pf · (inhabits · boolᶠ · x))))).
+Proof.
+intros P X M Pt Pf.
+reflexivity.
+Qed.
+
+Definition choice : El (
+  Πᶠ (A : El Typeᶠ) (B : El (A →ᶠ Typeᶠ)),
+    (Πᶠ x, [[ B · x ]]) →ᶠ
+    [[ Πᶠ x, B · x ]]
+).
+Proof.
+refine (λᶠ A B f, _).
+refine (exist _ _ _ tt).
+cbn; intros [x k].
+refine (f.(wit) (exist _ _ x k)).
+Defined.
+
+Definition rchoice : El (
+  Πᶠ (A : El Typeᶠ) (B : El (A →ᶠ Typeᶠ)),
+    [[ Πᶠ x, B · x ]]  →ᶠ
+    (Πᶠ x, [[ B · x ]])
+).
+Proof.
+refine (λᶠ A B f x, _).
+refine (exist _ _ _ tt).
+cbn; intros k.
+refine (f.(wit) (exist _ _ x k)).
+Defined.
+
+Lemma app_cc : forall (A B : El Typeᶠ) X (M : El (((A →ᶠ B) →ᶠ [[ X ]]) →ᶠ [[ A →ᶠ B ]])) (N : El A),
+  rchoice · A · (λᶠ (_ : El A), B) · (cc · (A →ᶠ B) · X · M) · N =
+    cc · B · X · (λᶠ (k : El (B →ᶠ [[ X ]])),
+      rchoice · A · (λᶠ (_ : El A), B) · (M · (λᶠ (f : El (A →ᶠ B)), k · (f · N))) · N).
+Proof.
+reflexivity.
+Qed.
+
 Inductive psigma (A : Type) (B : A -> Type) :=
 | pexist : forall x, B x -> psigma A B.
 
@@ -197,43 +246,14 @@ end
 ).
 Defined.
 
+(** Does not hold *)
 Definition choice : El (
   Πᶠ (A B : El Typeᶠ) (P : El (A →ᶠ B →ᶠ Typeᶠ)),
     (Πᶠ x, [[ sigmaᶠ · B · (λᶠ y, P · x · y) ]]) →ᶠ
     [[ sigmaᶠ · (A →ᶠ B) · (λᶠ f, Πᶠ x, P · x · (f · x)) ]]
 ).
 Proof.
-refine (λᶠ A B P f, _).
-revert f; intros [f _].
-unshelve refine (exist _ _ _ tt).
-cbn in *.
-refine (fun k => _).
-assert (k' := fun f y => k (pexist _ _ f y)); clear k; rename k' into k.
-cbn in *.
-assert (f' := fun x y => f (exist _ _ x y)); clear f; rename f' into f.
-cbn in *.
-
-unshelve refine (k _ _).
-+ unshelve refine (exist _ _ _ _).
-  - cbn; intros [x ω].
-    refine (f x _).
-    intros [y _]; refine (y.(wit) ω).
-  - intros x.
-cbn.
-
 Abort.
-
-Definition choice : El (
-  Πᶠ (A : El Typeᶠ) (B : El (A →ᶠ Typeᶠ)),
-    (Πᶠ x, [[ B · x ]]) →ᶠ
-    [[ Πᶠ x, B · x ]]
-).
-Proof.
-refine (λᶠ A B f, _).
-refine (exist _ _ _ tt).
-cbn; intros [x k].
-refine (f.(wit) (exist _ _ x k)).
-Defined.
 
 Inductive sum (A B : Type) :=
 | inl : A -> sum A B
@@ -258,3 +278,177 @@ cbn.
 refine (fun ω => ω (inr _ _ (λᶠ x, _))).
 destruct (ω (inl _ _ x)).
 Defined.
+
+Module Univ.
+
+Inductive path {A} (x : A) : A -> Type :=
+| refl : path x x.
+
+Definition isContr A := sig A (fun x => forall y, path x y).
+
+Definition fiber {A B} (f : A -> B) (y : B) : Type :=
+  sig A (fun x => path y (f x)).
+
+Definition isEquiv {A B} (f : A -> B) :=
+  forall y, isContr (fiber f y).
+
+Definition equiv A B := sig (A -> B) isEquiv.
+
+Definition Univalence := forall A, isContr (sig Type (fun X => equiv X A)).
+
+(*
+Definition idToEquiv A B (e : path A B) : sig :=
+  @path_rect Type A (fun B _ => A -> B) (fun x => x) B e.
+
+Definition Univalence := forall A B, @isEquiv (path A B) (A -> B) (idToEquiv A B).
+*)
+
+End Univ.
+
+Module Univᶠ.
+
+Inductive pathᵀ {A : El Typeᶠ} (x : El A) : El A -> Type :=
+| reflᵀ : pathᵀ x x.
+
+Inductive pathᴿ {A : El Typeᶠ} (x : El A) : forall y, M (pathᵀ x y) -> Type :=
+| reflᴿ : pathᴿ x x (ret (reflᵀ x)).
+
+Definition pathᶠ : El (Πᶠ (A : El Typeᶠ), A →ᶠ A →ᶠ Typeᶠ).
+Proof.
+refine (λᶠ A x y, _).
+refine (exist _ _ (ret _) (IsType _ (pathᴿ x y))).
+Defined.
+
+Definition reflᶠ : El (Πᶠ (A : El Typeᶠ) (x : El A), pathᶠ · A · x · x).
+Proof.
+refine (λᶠ (A : El Typeᶠ) (x : El A), _).
+refine (exist _ _ _ (reflᴿ _)).
+Defined.
+
+Definition path_rectᶠ :
+  El (Πᶠ (A : El Typeᶠ) (x : El A)
+    (P : El (Πᶠ (a : El A), pathᶠ · A · x · a →ᶠ Typeᶠ)),
+       P · x · (reflᶠ · A · x) →ᶠ Πᶠ (y : El A) (p : El (pathᶠ · A · x · y)), P · y · p).
+Proof.
+refine (λᶠ A x P p y e, _).
+destruct e as [? [ ] ].
+refine p.
+Defined.
+
+Definition isContrᶠ : El (Typeᶠ →ᶠ Typeᶠ) :=
+  λᶠ A, sigmaᶠ · A · (λᶠ x, Πᶠ (y : El A), pathᶠ · A · x · y).
+
+Definition fiberᶠ :
+  El (Πᶠ (A : El Typeᶠ) (B : El Typeᶠ), (A →ᶠ B) →ᶠ B →ᶠ Typeᶠ) :=
+  λᶠ A B f y, sigmaᶠ · A · (λᶠ x, pathᶠ · B · y · (f · x)).
+
+Definition isEquivᶠ :
+  El (Πᶠ (A : El Typeᶠ) (B : El Typeᶠ) (f : El (A →ᶠ B)), Typeᶠ) :=
+  λᶠ (A : El Typeᶠ) (B : El Typeᶠ) f, Πᶠ (y : El B), isContrᶠ · (fiberᶠ · A · B · f · y).
+
+Definition equivᶠ :=
+  λᶠ (A : El Typeᶠ) (B : El Typeᶠ),
+  sigmaᶠ · (A →ᶠ B) · (λᶠ f, isEquivᶠ · A · B · f).
+
+Definition Univalenceᶠ := Πᶠ (A : El Typeᶠ),
+  isContrᶠ · (sigmaᶠ · Typeᶠ · (λᶠ (X : El Typeᶠ), equivᶠ · X · A)).
+
+(*
+Definition idToEquivᶠ :=
+  λᶠ (A : El Typeᶠ) (B : El Typeᶠ) (e : El (pathᶠ · Typeᶠ · A · B)),
+  path_rectᶠ · Typeᶠ · A · (λᶠ (B : El Typeᶠ) _, A →ᶠ B) · (λᶠ (x : El A), x) · B · e.
+
+Definition Univalenceᶠ := Πᶠ (A : El Typeᶠ) (B : El Typeᶠ),
+  isEquivᶠ · (pathᶠ · Typeᶠ · A · B) · (A →ᶠ B) · (idToEquivᶠ · A · B).
+*)
+
+Lemma equiv_prod : forall A (B : El (A →ᶠ Typeᶠ)),
+  Univ.equiv (El (Πᶠ (x : El A), B · x)) (forall (x : El A), El (B · x)).
+Proof.
+intros A B.
+exists (fun f x => f · x).
+intros f.
+unshelve refine (exist _ _ _ _).
++ unshelve refine (exist _ _ (λᶠ x, f x) _).
+  reflexivity.
++ intros [g e].
+  refine (
+    match e in Univ.path _ h return
+      Univ.path
+        {|
+        wit := λᶠ x : El A, f x;
+        prf := Univ.refl (fun x : El A => (λᶠ x0 : El A, f x0) · x) |}
+      (exist _ _ (λᶠ x, h x) e)
+    with
+    | Univ.refl _ => _
+    end
+  ).
+reflexivity.
+Defined.
+
+Lemma path_sig : forall A (B : A -> Type) x₀ x₁ (y₀ : B x₀) (y₁ : B x₁)
+  (ex : Univ.path x₀ x₁)
+  (ey : match ex in Univ.path _ x return B x -> Type
+  with
+  | Univ.refl _ => fun y => Univ.path y₀ y
+  end y₁),
+  Univ.path (exist A B x₀ y₀) (exist A B x₁ y₁).
+Proof.
+intros.
+destruct ex.
+destruct ey.
+reflexivity.
+Defined.
+
+(*
+
+Lemma equiv_pathᵀ : forall (A : El Typeᶠ) (x y : El A),
+  Univ.equiv (@pathᵀ A x y) (@Univ.path (El A) x y).
+Proof.
+intros A x y.
+unshelve refine (exist _ _ _ _).
++ intros []; reflexivity.
++ intros e.
+  unshelve refine (exist _ _ _ _).
+  unshelve refine (exist _ _ _ _).
+  - destruct e; reflexivity.
+  - destruct e; reflexivity.
+  - intros [e' α].
+    destruct e.
+    unshelve refine (path_sig _ _ _ _ _ _ _ _).
+clear α.
+Defined.
+
+Lemma equiv_path : forall (A : El Typeᶠ) (x y : El A),
+  Univ.equiv (El (pathᶠ · A · x · y)) (@Univ.path (El A) x y).
+Proof.
+Abort.
+
+Lemma Univalence_preservation : Univ.Univalence -> El Univalenceᶠ.
+Proof.
+intros univ.
+refine (λᶠ A, _).
+unshelve refine (existᶠ · _ · _ · _ · _).
++ unshelve refine (existᶠ · _ · _ · A · _).
+  unshelve refine (existᶠ · _ · _ · (λᶠ (x : El A), x) · _).
+  refine (λᶠ x, _).
+  unshelve refine (existᶠ · _ · _ · (existᶠ · _ · _ · x · (reflᶠ · _ · x)) · _).
+  refine (λᶠ p, _).
+  refine (sigma_rectᶠ · _ · _ · _ · _ · p).
+  refine (λᶠ y q, _).
+  change (
+    El
+      (pathᶠ · (fiberᶠ · A · A · (λᶠ x : El A, x) · x)
+       · (existᶠ · A · (pathᶠ · A · x) · x · (reflᶠ · A · x))
+       · (existᶠ · A · (λᶠ y : El A, pathᶠ · A · x · y) · y
+          · q))
+  ).
+  refine (path_rectᶠ · A · x · (λᶠ y q, pathᶠ · (fiberᶠ · A · A · (λᶠ x : El A, x) · x)
+       · (existᶠ · A · (pathᶠ · A · x) · x · (reflᶠ · A · x))
+       · (existᶠ · A · (λᶠ y : El A, pathᶠ · A · x · y) · y
+          · q)) · _ · y · q).
+  refine (reflᶠ · _ · _).
++ refine (λᶠ X, _).
+
+
+Qed.
